examples/hwmcc_checker/aigScript.sml
@@ -223,6 +223,14 @@ Definition lit_map_def:
   lit_map f g h (v, b) = (var_map f g h v, b)
 End
 
+Theorem lit_map_o:
+  lit_map f g h ∘ lit_map f' g' h' = lit_map (f ∘ f') (g ∘ g') (h ∘ h')
+Proof
+  simp [FUN_EQ_THM] >> Cases >> simp [lit_map_def]
+  >> simp [oneline var_map_def, oneline bvar_map_def]
+  >> every_case_tac >> simp []
+QED
+
 Definition lit_map_base_def:
   lit_map_base f g = lit_map f g I
 End
