examples/hwmcc_checker/xaigScript.sml
@@ -108,10 +108,38 @@ Definition qxleft_def:
   qxleft (xaig: ('a, 'i, 'l) xaig) = xaig_map INL INL I xaig
 End
 
-Theorem xaig_map_cons[local]:
+Theorem xaig_map_nil[simp]:
+  xaig_map f g h [] = []
+Proof
+  simp [xaig_map_def]
+QED
+
+Theorem xaig_map_cons:
   xaig_map f g h (x::xaig) = gate_map f g h x::xaig_map f g h xaig
 Proof
   simp [xaig_map_def]
+QED
+
+Theorem gty_map_o:
+  gty_map f g h ∘ gty_map f' g' h' = gty_map (f ∘ f') (g ∘ g') (h ∘ h')
+Proof
+  simp [FUN_EQ_THM] >> Cases >> simp [gty_map_def]
+  >> simp [MAP_MAP_o, lit_map_o, SRULE [FUN_EQ_THM] lit_map_o]
+QED
+
+Theorem gate_map_o:
+  gate_map f g h ∘ gate_map f' g' h' = gate_map (f ∘ f') (g ∘ g') (h ∘ h')
+Proof
+  simp [FUN_EQ_THM] >> Cases >> simp [gate_map_def]
+  >> simp [SRULE [FUN_EQ_THM] gty_map_o]
+QED
+
+Theorem xaig_map_o:
+  xaig_map f g h ∘ xaig_map f' g' h' = xaig_map (f ∘ f') (g ∘ g') (h ∘ h')
+Proof
+  simp [FUN_EQ_THM] >> Induct >> simp []
+  >> simp [xaig_map_cons]
+  >> simp [SRULE [FUN_EQ_THM] gate_map_o]
 QED
 
 Theorem xaig_map_eq:
